     \chapter{Calculations}
     \label{ch:calcA6}
     
     \begin{equation}
V_{out-invert}=2\times V_{invert-ref}+(-1)\times (\frac{R_{F1}}{R_{in1}})\times V_{invert-in}
    \label{eq:invertB}
\end{equation}

\begin{equation}
    V_{invert-in}=\frac{R_2}{R_2+R_1}\times V_{bat}
    \label{eq:vinvertB}
\end{equation}

\begin{equation}
V_{non invert-out}= (1+\frac{R_{F2}}{R_{x}})\times V_{out-invert}
    \label{eq:noninvertB}
\end{equation}
     
     
     \centering Using eq.\ref{eq:vinvertB} and \ref{eq:invertB} the equation below is setup.
     \begin{center}
         $\frac{R_2}{R_1+R_2}=\frac{2\times V_{invert-ref} -283.3mV }{5.7}=\frac{2\times V_{invert-ref} -50mV }{7.5}$
     \end{center}
     \centering $V_{invert-ref}=511mV$
     \centering $R_1$ chosen to be 180k and $R_2=26.8$k\textohm(lab resistor is 27k\textohm)




